ProgramHyperproperties.thy
@@ -10,20 +10,142 @@ definition set_of_traces where
 definition hypersat :: "pproc \<Rightarrow> progran_hyperproperty \<Rightarrow> bool" where
   "hypersat C H \<longleftrightarrow> H {(s, l, s') |s l s'. par_big_step C s l s'}"
 
-theorem proving_hyperproperties:
-  "\<exists>P Q. (\<forall>C. hypersat C H \<longleftrightarrow> \<Turnstile>\<^sub>P {P} C {Q})"
-proof-
-  let ?P = "\<lambda>S. S = {s :: gstate |s. True}"
-  let ?Q = "\<lambda>S. H {(s, l ,s') |s s' l. (s', l) \<in> S}"
+definition injective where
+  "injective f \<longleftrightarrow> (\<forall>a b. a \<noteq> b \<longrightarrow> f a \<noteq> f b)"
 
-  have "\<And>C. hypersat C H \<longleftrightarrow> \<Turnstile>\<^sub>P {?P} C {?Q}"
+definition copy_p_state where
+  "copy_p_state to_pvar to_lval \<sigma> x = to_lval (\<sigma> (to_pvar x))"
+
+definition recover_p_state where
+  "recover_p_state to_pval to_lvar l x = to_pval (l (to_lvar x))"
+
+lemma injective_then_exists_inverse:
+  assumes "injective to_lvar"
+  shows "\<exists>to_pvar. (\<forall>x. to_pvar (to_lvar x) = x)"
+proof -
+  let ?to_pvar = "\<lambda>y. SOME x. to_lvar x = y"
+  have "\<And>x. ?to_pvar (to_lvar x) = x"
+    by (metis (mono_tags, lifting) assms injective_def someI)
+  then show ?thesis
+    by force
+qed
+
+lemma in_set_of_traces_then_in_sem:
+  assumes "(s\<^sub>p, l, s\<^sub>p') \<in> set_of_traces C"
+      and "(s\<^sub>l, s\<^sub>p) \<in> S"
+    shows "(s\<^sub>l, s\<^sub>p', l) \<in> par_sem C S"
+  using assms(1) assms(2) in_par_sem set_of_traces_def by fastforce
+
+lemma set_of_single_traces_same:
+  assumes "\<And>x. to_pvar (to_lvar x) = x"
+      and "\<And>x. to_pval (to_lval x) = x"
+      and "S = {(copy_p_state to_pvar to_lval \<sigma>\<^sub>p, State \<sigma>\<^sub>p) |\<sigma>\<^sub>p. True}"
+    shows "{(State (recover_p_state to_pval to_lvar \<sigma>\<^sub>l), l, State \<sigma>\<^sub>p') |\<sigma>\<^sub>l \<sigma>\<^sub>p' l. (\<sigma>\<^sub>l, State \<sigma>\<^sub>p', l) \<in> par_sem (Single C) S} = set_of_traces (Single C)"
+(is "?A = ?B")
+proof
+  show "?A \<subseteq> ?B"
+  proof (rule subsetTupleI)
+    fix s\<^sub>p s\<^sub>p' l assume asm0: "(s\<^sub>p, l, s\<^sub>p') \<in> ?A"
+    then obtain \<sigma>\<^sub>l \<sigma>\<^sub>p' where asm1: "s\<^sub>p = State (recover_p_state to_pval to_lvar \<sigma>\<^sub>l)" 
+    "(\<sigma>\<^sub>l, State \<sigma>\<^sub>p', l) \<in> par_sem (Single C) S" "s\<^sub>p' = State \<sigma>\<^sub>p'"
+      by blast
+    then obtain \<sigma>\<^sub>p where "(\<sigma>\<^sub>l, State \<sigma>\<^sub>p) \<in> S" "big_step C \<sigma>\<^sub>p l \<sigma>\<^sub>p'"
+      by (smt (verit, del_insts) SingleE fst_conv gstate.inject(1) in_par_sem snd_conv)     
+    then have "\<sigma>\<^sub>l = copy_p_state to_pvar to_lval \<sigma>\<^sub>p"
+      using assms(3) by blast
+    moreover have "s\<^sub>p = State \<sigma>\<^sub>p"
+      sledgehammer
+    proof -
+      have f1: "\<forall>f fa fb a. copy_p_state fb f fa (a::'a) = (f (fa (fb a::char)::real)::'b)"
+        by (simp add: copy_p_state_def)
+      have f2: "\<forall>f fa fb c. recover_p_state f fb fa (c::char) = (f (fa (fb c::'a)::'b)::real)"
+        by (simp add: recover_p_state_def)
+      obtain bb :: "'a \<Rightarrow> 'b" where
+        f3: "s\<^sub>p = State (recover_p_state to_pval to_lvar bb) \<and> s\<^sub>p = State (recover_p_state to_pval to_lvar bb)"
+        using \<open>\<And>thesis. (\<And>\<sigma>\<^sub>l \<sigma>\<^sub>p'. \<lbrakk>s\<^sub>p = State (recover_p_state to_pval to_lvar \<sigma>\<^sub>l); (\<sigma>\<^sub>l, State \<sigma>\<^sub>p', l) \<in> par_sem (Single C) S; s\<^sub>p' = State \<sigma>\<^sub>p'\<rbrakk> \<Longrightarrow> thesis) \<Longrightarrow> thesis\<close> by moura
+      then have "State (recover_p_state to_pval to_lvar bb) = State (recover_p_state to_pval to_lvar (copy_p_state to_pvar to_lval \<sigma>\<^sub>p))"
+        using asm1(1) calculation by argo
+      then show ?thesis
+        using f3 f2 f1 assms(1) assms(2) by fastforce
+    qed
+    ultimately show "(s\<^sub>p, l, s\<^sub>p') \<in> ?B"
+      by (simp add: SingleB \<open>big_step C \<sigma>\<^sub>p l \<sigma>\<^sub>p'\<close> \<open>s\<^sub>p' = State \<sigma>\<^sub>p'\<close> set_of_traces_def)
+  qed
+  show "?B \<subseteq> ?A"
+  proof (rule subsetTupleI)
+    fix s\<^sub>p s\<^sub>p' l assume asm0: "(s\<^sub>p, l, s\<^sub>p') \<in> ?B"
+    then obtain \<sigma>\<^sub>p \<sigma>\<^sub>p' where asm1: "s\<^sub>p = State \<sigma>\<^sub>p" "s\<^sub>p' = State \<sigma>\<^sub>p'" "big_step C \<sigma>\<^sub>p l \<sigma>\<^sub>p'"
+      by (smt (verit) Pair_inject SingleE mem_Collect_eq set_of_traces_def)
+    let ?\<sigma>\<^sub>l = "copy_p_state to_pvar to_lval \<sigma>\<^sub>p"
+    have "(?\<sigma>\<^sub>l, State \<sigma>\<^sub>p) \<in> S"
+      using assms(3) by blast
+    then have "(?\<sigma>\<^sub>l, State \<sigma>\<^sub>p', l) \<in> par_sem (Single C) S"
+      using asm0 asm1 in_set_of_traces_then_in_sem by blast
+    moreover have "recover_p_state to_pval to_lvar ?\<sigma>\<^sub>l = \<sigma>\<^sub>p"
+    proof -
+      have f1: "\<forall>f fa fb a. copy_p_state fb f fa (a::'a) = (f (fa (fb a::char)::real)::'b)"
+        by (meson copy_p_state_def)
+      have "\<forall>f fa fb c. recover_p_state f fb fa (c::char) = (f (fa (fb c::'a)::'b)::real)"
+        by (simp add: recover_p_state_def)
+      then show ?thesis
+        using f1 assms(1) assms(2) by auto
+    qed
+    ultimately show "(s\<^sub>p, l, s\<^sub>p') \<in> ?A"
+      using asm1(1) asm1(2) by force
+    qed
+  qed
+
+
+theorem proving_hyperproperties:
+
+  fixes to_lvar :: " var \<Rightarrow> 'lvar"
+  fixes to_lval :: " real \<Rightarrow> 'lval"
+
+  assumes "injective to_lvar"
+      and "injective to_lval"
+
+shows "\<exists>P :: (('lvar, 'lval) lstate \<times> gstate) set \<Rightarrow> bool. 
+       \<exists>Q :: (('lvar, 'lval) lstate \<times> gstate \<times> trace) set \<Rightarrow> bool. 
+       (\<forall>C. hypersat (Single C) H \<longleftrightarrow> \<Turnstile>\<^sub>P {P} (Single C) {Q})"
+proof-
+
+  obtain to_pval :: "'lval \<Rightarrow> real" where r1: "\<And>x. to_pval (to_lval x) = x"
+    using assms(2) injective_then_exists_inverse by blast
+
+  obtain to_pvar :: "'lvar \<Rightarrow> var" where r2: "\<And>x. to_pvar (to_lvar x) = x"
+    using assms(1) injective_then_exists_inverse by blast
+
+  let ?P = "\<lambda>S. S = {(copy_p_state to_pvar to_lval \<sigma>\<^sub>p, State \<sigma>\<^sub>p) |\<sigma>\<^sub>p. True}"
+  let ?Q = "\<lambda>S. H {(State (recover_p_state to_pval to_lvar \<sigma>\<^sub>l), l, State \<sigma>\<^sub>p') |\<sigma>\<^sub>l \<sigma>\<^sub>p' l. (\<sigma>\<^sub>l , State \<sigma>\<^sub>p', l) \<in> S }"
+
+  have "\<And>C. hypersat (Single C) H \<longleftrightarrow> \<Turnstile>\<^sub>P {?P} (Single C) {?Q}"
   proof
     fix C
-    assume "hypersat C H"
-    show "\<Turnstile>\<^sub>P {?P} C {?Q}"
+    assume "hypersat (Single C) H"
+    show "\<Turnstile>\<^sub>P {?P} (Single C) {?Q}"
     proof (rule par_hyper_hoare_tripleI)
-
-        
+      fix S assume "S = {(copy_p_state to_pvar to_lval \<sigma>\<^sub>p, State \<sigma>\<^sub>p) |\<sigma>\<^sub>p. True}"
+      have "{(State (recover_p_state to_pval to_lvar \<sigma>\<^sub>l), l, State \<sigma>\<^sub>p') |\<sigma>\<^sub>l \<sigma>\<^sub>p' l. (\<sigma>\<^sub>l, State \<sigma>\<^sub>p', l) \<in> par_sem (Single C) S} = set_of_traces (Single C)"
+        using \<open>S = {(copy_p_state to_pvar to_lval \<sigma>\<^sub>p, State \<sigma>\<^sub>p) |\<sigma>\<^sub>p. True}\<close> set_of_single_traces_same[of to_pvar to_lvar to_pval to_lval]
+        r1 r2 by auto
+      then show "H {(State (recover_p_state to_pval to_lvar \<sigma>\<^sub>l), l, State \<sigma>\<^sub>p') |\<sigma>\<^sub>l \<sigma>\<^sub>p' l. (\<sigma>\<^sub>l, State \<sigma>\<^sub>p', l) \<in> par_sem (Single C) S}"
+        by (smt (verit, best) Collect_cong \<open>hypersat (Single C) H\<close> hypersat_def set_of_traces_def)
+    qed
+  next
+    fix C
+    let ?S = "{(copy_p_state to_pvar to_lval \<sigma>\<^sub>p, State \<sigma>\<^sub>p) |\<sigma>\<^sub>p. True }"
+    assume "\<Turnstile>\<^sub>P {?P} (Single C) {?Q}"
+    then have "?Q (par_sem (Single C) ?S)"
+      using par_hyper_hoare_tripleE by blast
+    moreover have "{(State (recover_p_state to_pval to_lvar \<sigma>\<^sub>l), l, State \<sigma>\<^sub>p') |\<sigma>\<^sub>l \<sigma>\<^sub>p' l. (\<sigma>\<^sub>l, State \<sigma>\<^sub>p', l) \<in> par_sem (Single C) ?S} = set_of_traces (Single C)"
+      using r1 r2 set_of_single_traces_same[of to_pvar to_lvar to_pval to_lval]
+      by presburger
+    ultimately show "hypersat (Single C) H"
+      by (smt (verit, best) Collect_cong hypersat_def set_of_traces_def)
+  qed
+  then show ?thesis
+    by blast
+qed
 
 definition semify where
   "semify \<Sigma> S = { (s', l) |s' s l. s \<in> S \<and> (s, l, s') \<in> \<Sigma> }"
